Aoc2023/AesopExtra.lean
@@ -1,0 +1,12 @@
+import Aesop
+
+--@[aesop safe forward]
+--theorem Nat.eq_of_le_of_not_lt {n m : Nat} (h₁ : n ≤ m) (h₂ : ¬(n < m)) : n = m :=
+--  Or.casesOn (Nat.eq_or_lt_of_le h₁) id (fun h => False.elim <| h₂ h)
+
+@[aesop safe forward]
+theorem Nat.eq_of_le_of_le {n m : Nat} (h₁ : n ≤ m) (h₂ : m ≤ n) : n = m := by
+  simp [Nat.le_antisymm_iff, h₁, h₂]
+
+attribute [aesop safe forward] Nat.le_of_lt_succ
+
