Aoc2023/Day08.lean
@@ -1,0 +1,33 @@
+import Aoc2023.Utils
+
+open System Lean Lean.Parsec
+
+namespace Day08
+
+def testinput : FilePath := "/home/fred/lean/aoc2023/input_08_test"
+def testinput2 : FilePath := "/home/fred/lean/aoc2023/input_08_test2"
+def realinput : FilePath := "/home/fred/lean/aoc2023/input_08"
+
+/-
+PART 1:
+-/
+
+def firstPart (input : FilePath) : IO Nat := do
+  let rawdata := (← IO.FS.lines input)
+  return 0
+
+--#eval firstPart testinput           --(ans: )
+--#eval firstPart realinput           --(ans: )
+
+/-
+PART 2:
+-/
+
+def secondPart (input : FilePath) : IO Nat := do
+  let rawdata := (← IO.FS.lines input)
+  return 0
+
+--#eval secondPart testinput           --(ans: )
+--#eval secondPart realinput           --(ans: )
+
+end Day08
