Main.lean
@@ -5,6 +5,7 @@ import Aoc2023.Day04
 import Aoc2023.Day05
 import Aoc2023.Day06
 import Aoc2023.Day07
+import Aoc2023.Day08
 
 def main (args : List String) : IO Unit :=
   match args with
@@ -41,7 +42,12 @@ def main (args : List String) : IO Unit :=
   | ["7"] => do
     IO.println "Day 7:"
     IO.println s!"Part 1: {← Day07.firstPart "input_07"}"
-    IO.println s!"Part 2: {← Day07.secondPart "input_07"}"
+    --IO.println s!"Part 2: {← Day07.secondPart "input_07"}"
+    IO.println ""
+  | ["8"] => do
+    IO.println "Day 8:"
+    IO.println s!"Part 1: {← Day08.firstPart "input_08"}"
+    IO.println s!"Part 2: {← Day08.secondPart "input_08"}"
     IO.println ""
   | _ => do
     IO.println "Help, what should I do!?"
